SepLogic/Hoare_Triple.thy
@@ -1,0 +1,185 @@
+theory Hoare_Triple
+imports Run
+begin
+
+section {* Definition of hoare triple, and the frame rule. *}
+
+text {* Analyze the heap before and after executing a command, to add
+  the allocated addresses to the covered address range. *}
+
+definition new_addrs :: "heap \<Rightarrow> addr set \<Rightarrow> heap \<Rightarrow> addr set" where
+  "new_addrs h as h' = as \<union> {a. lim h \<le> a \<and> a < lim h'}"
+setup {* add_rewrite_rule @{thm new_addrs_def} *}
+
+lemma new_addr_refl [rewrite]: "new_addrs h as h = as" by auto2
+
+definition hoare_triple :: "assn \<Rightarrow> 'a Heap \<Rightarrow> ('a \<Rightarrow> assn) \<Rightarrow> bool" ("<_>/ _/ <_>") where
+  "<P> c <Q> \<longleftrightarrow> (\<forall>h as \<sigma> r. (h, as) \<Turnstile> P \<longrightarrow> run c (Some h) \<sigma> r \<longrightarrow>
+    (\<sigma> \<noteq> None \<and> (the \<sigma>, new_addrs h as (the \<sigma>)) \<Turnstile> Q r \<and> relH {a . a < lim h \<and> a \<notin> as} h (the \<sigma>) \<and>
+     lim h \<le> lim (the \<sigma>)))"
+setup {* add_forward_prfstep (equiv_forward_th @{thm hoare_triple_def}) *}
+setup {* add_resolve_prfstep (equiv_backward_th @{thm hoare_triple_def}) *}
+
+text {* For garbage-collected languages, specifications usually allow for some
+  arbitrary heap parts in the postcondition. The following abbreviation defines
+  a handy shortcut notation for such specifications. *}
+abbreviation hoare_triple' :: "assn \<Rightarrow> 'r Heap \<Rightarrow> ('r \<Rightarrow> assn) \<Rightarrow> bool" ("<_> _ <_>\<^sub>t") where
+  "<P> c <Q>\<^sub>t \<equiv> <P> c <\<lambda>r. Q r * true>"
+
+setup {* add_rewrite_rule @{thm disjoint_with_union} *}
+lemma frame_rule [backward]:
+  "<P> c <Q> \<Longrightarrow> <P * R> c <\<lambda>x. Q x * R>"
+  by (tactic {* auto2s_tac @{context}
+    (OBTAIN ("\<forall>h as \<sigma> r. (h, as) \<Turnstile> P * R \<longrightarrow> run c (Some h) \<sigma> r \<longrightarrow>" ^
+                "(\<sigma> \<noteq> None \<and> (the \<sigma>, new_addrs h as (the \<sigma>)) \<Turnstile> Q r * R \<and> relH {a . a < lim h \<and> a \<notin> as} h (the \<sigma>) \<and>" ^
+                "lim h \<le> lim (the \<sigma>))") WITH (
+       CHOOSE "as1, as2, set_partition as as1 as2 \<and> (h, as1) \<Turnstile> P \<and> (h, as2) \<Turnstile> R" THEN
+       OBTAIN "relH as2 h (the \<sigma>)" THEN
+       OBTAIN "set_partition (new_addrs h as (the \<sigma>)) (new_addrs h as1 (the \<sigma>)) as2" WITH
+         OBTAIN "\<forall>x. x \<in> as2 \<longrightarrow> x \<notin> {a. lim h \<le> a \<and> a < lim (the \<sigma>)}")) *})
+setup {* del_prfstep_thm @{thm disjoint_with_union} *}
+
+(* This is the last use of the definition of separating conjunction. *)
+setup {* del_prfstep_thm @{thm mod_star_conv} *}
+setup {* del_prfstep "Hoare_Triple.hoare_triple_def@eqbackward@res" *}
+
+section {* Hoare triples for atomic commands *}
+
+setup {* add_backward_prfstep (equiv_backward_th @{thm hoare_triple_def}) *}
+(* First, those that do not modify the heap. *)
+lemma return_rule:
+  "<emp> return x <\<lambda>r. \<up>(r = x)>" by auto2
+
+lemma nth_rule:
+  "<a \<mapsto>\<^sub>a xs * \<up>(i < length xs)> Array.nth a i <\<lambda>r. a \<mapsto>\<^sub>a xs * \<up>(r = xs ! i)>" by auto2
+
+lemma length_rule:
+  "<a \<mapsto>\<^sub>a xs> Array.len a <\<lambda>r. a \<mapsto>\<^sub>a xs * \<up>(r = length xs)>" by auto2
+
+lemma lookup_rule:
+  "<p \<mapsto>\<^sub>r x> !p <\<lambda>r. p \<mapsto>\<^sub>r x * \<up>(r = x)>" by auto2
+
+(* Next, the update rules. *)
+setup {* add_rewrite_rule @{thm Ref.lim_set} *}
+theorem Array_lim_set [rewrite]: "lim (Array.set p xs h) = lim h" by (simp add: Array.set_def)
+
+setup {* fold add_rewrite_rule [@{thm Ref.get_set_eq}, @{thm Array.get_set_eq}] *}
+setup {* add_rewrite_rule @{thm Array.update_def} *}
+
+lemma upd_rule:
+  "<a \<mapsto>\<^sub>a xs * \<up>(i < length xs)> Array.upd i x a <\<lambda>r. a \<mapsto>\<^sub>a list_update xs i x * \<up>(r = a)>" by auto2
+
+lemma update_rule:
+  "<p \<mapsto>\<^sub>r y> p := x <\<lambda>r. p \<mapsto>\<^sub>r x>" by auto2
+
+(* Finally, the allocation rules. *)
+theorem lim_set_gen [rewrite]: "lim (h\<lparr>lim := l\<rparr>) = l" by simp
+
+theorem Array_alloc_def' [rewrite]: 
+  "Array.alloc xs h = (let l = lim h; r = Array l in (r, (Array.set r xs (h\<lparr>lim := l + 1\<rparr>))))"
+  by (simp add: Array.alloc_def)
+
+setup {* fold add_rewrite_rule [
+  @{thm addr_of_array.simps}, @{thm addr_of_ref.simps}, @{thm Ref.alloc_def}] *}
+
+theorem refs_on_Array_set [rewrite]: "refs (Array.set p xs h) t i = refs h t i"
+  by (simp add: Array.set_def)
+
+theorem arrays_on_Ref_set [rewrite]: "arrays (Ref.set p x h) t i = arrays h t i"
+  by (simp add: Ref.set_def)
+
+theorem refs_on_Array_alloc [rewrite]: "refs (snd (Array.alloc xs h)) t i = refs h t i"
+  by (metis (no_types, lifting) Array.alloc_def refs_on_Array_set select_convs(2) snd_conv surjective update_convs(3))
+
+theorem arrays_on_Ref_alloc [rewrite]: "arrays (snd (Ref.alloc x h)) t i = arrays h t i"
+  by (metis (no_types, lifting) Ref.alloc_def arrays_on_Ref_set select_convs(1) sndI surjective update_convs(3))
+
+theorem arrays_on_Array_alloc [rewrite]: "i < lim h \<Longrightarrow> arrays (snd (Array.alloc xs h)) t i = arrays h t i"
+  by (smt Array.alloc_def Array.set_def addr_of_array.simps fun_upd_apply less_or_eq_imp_le
+          linorder_not_less simps(1) snd_conv surjective update_convs(1) update_convs(3))
+
+theorem refs_on_Ref_alloc [rewrite]: "i < lim h \<Longrightarrow> refs (snd (Ref.alloc x h)) t i = refs h t i"
+  by (smt Ref.alloc_def Ref.set_def addr_of_ref.simps fun_upd_apply less_or_eq_imp_le
+          linorder_not_less select_convs(2) simps(6) snd_conv surjective update_convs(3))
+
+lemma new_rule:
+  "<emp> Array.new n x <\<lambda>r. r \<mapsto>\<^sub>a replicate n x>" by auto2
+
+lemma ref_rule:
+  "<emp> ref x <\<lambda>r. r \<mapsto>\<^sub>r x>" by auto2
+
+setup {* fold del_prfstep_thm [@{thm sngr_assn_rule}, @{thm snga_assn_rule}] *}
+
+section {* Other properties *}
+
+theorem norm_pre_pure_iff: "<P * \<up>b> c <Q> \<longleftrightarrow> (b \<longrightarrow> <P> c <Q>)" by auto2
+theorem norm_pre_pure_iff_sng: "<\<up>b> c <Q> \<longleftrightarrow> (b \<longrightarrow> <emp> c <Q>)" by auto2
+
+section {* success_run and its properties. *}
+
+theorem union_case [forward]: "x \<in> A \<union> B \<Longrightarrow> x \<in> A \<or> x \<in> B" by auto2
+theorem new_addrs_bind [rewrite]: "lim h \<le> lim h' \<Longrightarrow> lim h' \<le> lim h'' \<Longrightarrow>
+  new_addrs h' (new_addrs h as h') h'' = new_addrs h as h''"
+  by (tactic {* auto2s_tac @{context}
+    (OBTAIN "\<forall>x. x \<in> new_addrs h' (new_addrs h as h') h'' \<longleftrightarrow> x \<in> new_addrs h as h''") *})
+setup {* del_prfstep_thm @{thm union_case} *}
+
+definition success_run :: "'a Heap \<Rightarrow> heap \<Rightarrow> nat set \<Rightarrow> heap \<Rightarrow> nat set \<Rightarrow> 'a \<Rightarrow> bool" where
+  "success_run f h as h' as' r \<longleftrightarrow>
+    as' = new_addrs h as h' \<and> run f (Some h) (Some h') r \<and> relH {a. a < lim h \<and> a \<notin> as} h h' \<and> lim h \<le> lim h'"
+setup {* add_rewrite_rule @{thm success_run_def} *}
+
+theorem success_run_bind:
+  "success_run f h as h' as' r \<Longrightarrow> success_run (g r) h' as' h'' as'' r' \<Longrightarrow>
+   success_run (f \<bind> g) h as h'' as'' r'" by auto2
+
+theorem success_run_next: "success_run f h as h'' as'' r' \<Longrightarrow>
+  \<forall>h' as'. \<sigma> = Some h' \<and> success_run (f \<bind> g) h as h' as' r \<longrightarrow> \<not> (h', as') \<Turnstile> Q \<Longrightarrow>
+  \<forall>h' as'. \<sigma> = Some h' \<and> success_run (g r') h'' as'' h' as' r \<longrightarrow> \<not> (h', as') \<Turnstile> Q" by auto2
+
+theorem hoare_tripleE': "<P> c <Q> \<Longrightarrow> (h, as) \<Turnstile> P * Ru \<Longrightarrow> run c (Some h) \<sigma> r \<Longrightarrow>
+  \<exists>h' as'. (h', as') \<Turnstile> Q r * Ru \<and> \<sigma> = Some h' \<and> success_run c h as h' as' r"
+  by (tactic {* auto2s_tac @{context}
+    (OBTAIN "<P * Ru> c <\<lambda>r. Q r * Ru>" THEN OBTAIN "\<sigma> \<noteq> None") *})
+
+theorem hoare_tripleI: "\<not><P> c <Q> \<Longrightarrow> \<exists>h as \<sigma> r. (h, as) \<Turnstile> P \<and> run c (Some h) \<sigma> r \<and>
+  (\<forall>h' as'. \<sigma> = Some h' \<and> success_run c h as h' as' r \<longrightarrow> \<not>(h', as') \<Turnstile> Q r)" by auto2
+
+theorem hoare_triple_mp:
+  "<P> c <Q> \<Longrightarrow> (h, as) \<Turnstile> P * Ru \<Longrightarrow> success_run c h as h' as' r \<Longrightarrow> (h', as') \<Turnstile> (Q r) * Ru"
+  by (tactic {* auto2s_tac @{context} (OBTAIN "<P * Ru> c <\<lambda>r. Q r * Ru>") *})
+
+theorem hoare_tripleE'': "<P> c <Q> \<Longrightarrow> (h, as) \<Turnstile> P * Ru \<Longrightarrow> run (c \<bind> g) (Some h) \<sigma> r \<Longrightarrow>
+  \<exists>r' h' as'. run (g r') (Some h') \<sigma> r \<and> (h', as') \<Turnstile> Q r' * Ru \<and> success_run c h as h' as' r'"
+  by (tactic {* auto2s_tac @{context}
+    (OBTAIN "<P * Ru> c <\<lambda>r. Q r * Ru>" THEN
+     CHOOSE "\<sigma>', r', run c (Some h) \<sigma>' r'" THEN OBTAIN "\<sigma>' \<noteq> None") *})
+
+definition heap_preserving :: "'a Heap \<Rightarrow> bool" where
+  "heap_preserving c = (\<forall>h h' r. effect c h h' r \<longrightarrow> h = h')"
+setup {* add_rewrite_rule @{thm heap_preserving_def} *}
+
+setup {* add_forward_prfstep @{thm effectI} *}
+
+theorem heap_preservingD [forward]:
+  "heap_preserving c \<Longrightarrow> success_run c h as h' as' r \<Longrightarrow> h = h' \<and> as = as'" by auto2
+
+theorem heap_preserving_effectD:
+  "heap_preserving c \<Longrightarrow> effect c h h' r \<Longrightarrow> h = h'" by auto2
+
+theorem effect_bind [forward]: "effect (f \<bind> g) h h'' r' \<Longrightarrow> \<exists>h' r. effect f h h' r \<and> effect (g r) h' h'' r'"
+  by (elim effect_elims) auto
+
+theorem hoare_tripleE'_preserve: "heap_preserving c \<Longrightarrow>
+  \<exists>h' as'. (h', as') \<Turnstile> Q \<and> \<sigma> = Some h' \<and> success_run c h as h' as' r \<Longrightarrow>
+  (h, as) \<Turnstile> Q \<and> \<sigma> = Some h \<and> success_run c h as h as r" by auto2
+
+theorem hoare_tripleE''_preserve: "heap_preserving c \<Longrightarrow>
+  \<exists>r' h' as'. run (g r') (Some h') \<sigma> r \<and> (h', as') \<Turnstile> Q r' * Ru \<and> success_run c h as h' as' r' \<Longrightarrow>
+  \<exists>r'. run (g r') (Some h) \<sigma> r \<and> (h, as) \<Turnstile> Q r' * Ru \<and> success_run c h as h as r'" by auto2
+
+setup {* del_prfstep_thm @{thm effectI} *}
+setup {* del_prfstep_thm @{thm hoare_triple_def} *}
+setup {* del_prfstep_thm @{thm surjective_pairing} *}
+
+end
