SepLogic/RBT.thy
@@ -1,0 +1,661 @@
+(* Red-black trees. *)
+
+theory RBT
+imports SepAuto Mapping
+begin
+
+section {* Abstract red-black trees *}
+
+datatype color = R | B
+
+datatype ('a, 'b) rbt =
+  Leaf | Node (lsub: "('a, 'b) rbt") (cl: color) (key: 'a) (val: 'b) (rsub: "('a, 'b) rbt")
+where
+  "cl Leaf = B"
+
+setup {* add_resolve_prfstep @{thm color.distinct(1)} *}
+setup {* add_resolve_prfstep @{thm rbt.distinct(2)} *}
+setup {* fold add_rewrite_rule @{thms rbt.sel} *}
+setup {* add_forward_prfstep (equiv_forward_th (@{thm rbt.simps(1)})) *}
+
+text {* Case checking for trees: first verify the Tip case, then can assume t is
+  in the form Node l c k v r. *}
+
+setup {* add_gen_prfstep ("rbt_case_intro",
+  [WithTerm @{term_pat "?t::(?'a, ?'b) rbt"},
+   Filter (unique_free_filter "t"),
+   CreateCase @{term_pat "(?t::(?'a, ?'b) rbt) = Leaf"}]) *}
+setup {* add_forward_prfstep_cond @{thm rbt.collapse} [with_cond "?rbt \<noteq> Node ?l ?c ?k ?v ?r"] *}
+
+text {* Induction on trees: after checking Tip case, can assume P (lsub t)
+  and P (rsub t) holds when trying to prove P t. *}
+
+theorem rbt_induct': "P Leaf \<Longrightarrow> (\<forall>t. P (lsub t) \<and> P (rsub t) \<longrightarrow> P t) \<Longrightarrow> P t"
+  apply (induction t) apply blast by (metis rbt.sel(1) rbt.sel(6))
+setup {* add_prfstep_induction @{thm rbt_induct'} *}
+
+subsection {* Some trivial lemmas *}
+
+theorem not_R [forward]: "c \<noteq> R \<Longrightarrow> c = B" using color.exhaust by blast
+theorem not_B [forward]: "c \<noteq> B \<Longrightarrow> c = R" using color.exhaust by blast
+theorem red_not_leaf [forward]: "cl t = R \<Longrightarrow> t \<noteq> Leaf" by auto
+theorem if_not_Leaf [rewrite]: "(if Node l c k v r = Leaf then a else b) = b" by simp
+theorem if_R [rewrite]: "(if R = B then a else b) = b" by simp
+theorem if_B [rewrite]: "(if B = R then a else b) = b" by simp
+
+subsection {* Definition of main functions and invariants *}
+
+fun min_depth :: "('a, 'b) rbt \<Rightarrow> nat" where
+  "min_depth Leaf = 0"
+| "min_depth (Node l c k v r) = min (min_depth l) (min_depth r) + 1"
+
+fun max_depth :: "('a, 'b) rbt \<Rightarrow> nat" where
+  "max_depth Leaf = 0"
+| "max_depth (Node l c k v r) = max (max_depth l) (max_depth r) + 1"
+
+fun black_depth :: "('a, 'b) rbt \<Rightarrow> nat" where
+  "black_depth Leaf = 0"
+| "black_depth (Node l R k v r) = min (black_depth l) (black_depth r)"
+| "black_depth (Node l B k v r) = min (black_depth l) (black_depth r) + 1"
+
+fun cl_inv :: "('a, 'b) rbt \<Rightarrow> bool" where
+  "cl_inv Leaf = True"
+| "cl_inv (Node l R k v r) = (cl_inv l \<and> cl_inv r \<and> cl l = B \<and> cl r = B)"
+| "cl_inv (Node l B k v r) = (cl_inv l \<and> cl_inv r)"
+
+fun bd_inv :: "('a, 'b) rbt \<Rightarrow> bool" where
+  "bd_inv Leaf = True"
+| "bd_inv (Node l c k v r) = (bd_inv l \<and> bd_inv r \<and> black_depth l = black_depth r)"
+
+definition is_rbt :: "('a, 'b) rbt \<Rightarrow> bool" where
+  "is_rbt t = (cl_inv t \<and> bd_inv t)"
+
+setup {* fold add_rewrite_rule (
+  @{thms min_depth.simps} @ @{thms max_depth.simps} @ @{thms black_depth.simps} @
+  @{thms cl_inv.simps} @ @{thms bd_inv.simps} @ [@{thm is_rbt_def}]) *}
+theorem cl_invI: "cl_inv l \<Longrightarrow> cl_inv r \<Longrightarrow> cl_inv (Node l B k v r)" by auto
+setup {* add_forward_prfstep_cond @{thm cl_invI} [with_term "cl_inv (Node ?l B ?k ?v ?r)"] *}
+
+subsection {* Properties of bd_inv *}
+
+theorem bd_inv_elimR [rewrite]:
+  "bd_inv (Node l R k v r) \<Longrightarrow> black_depth (Node l R k v r) = black_depth l" by auto2
+theorem bd_inv_elimB [rewrite]:
+  "bd_inv (Node l B k v r) \<Longrightarrow> black_depth (Node l B k v r) = black_depth l + 1" by auto2
+theorem bd_inv_intro: "black_depth l = black_depth r \<Longrightarrow> bd_inv l \<Longrightarrow> bd_inv r \<Longrightarrow> bd_inv (Node l c k v r)" by auto2
+setup {* add_forward_prfstep_cond @{thm bd_inv_intro} [with_term "Node ?l ?c ?k ?v ?r"] *}
+
+subsection {* is_rbt is recursive *}
+
+theorem is_rbt_rec [forward]: "is_rbt (Node l c k v r) \<Longrightarrow> is_rbt l \<and> is_rbt r"
+  by (tactic {* auto2s_tac @{context} (CASE "c = R") *})
+
+subsection {* Balancedness of is_rbt *}
+
+theorem depth_min: "is_rbt t \<Longrightarrow> black_depth t \<le> min_depth t"
+  by (tactic {* auto2s_tac @{context}
+    (CASE "t = Leaf" THEN
+     CASE "cl t = R" WITH
+        OBTAIN "black_depth t \<le> min (min_depth (lsub t)) (min_depth (rsub t))") *} )
+
+theorem depth_max: "is_rbt t \<Longrightarrow> if cl t = R then max_depth t \<le> 2 * black_depth t + 1
+                                 else max_depth t \<le> 2 * black_depth t"
+  by (tactic {* auto2s_tac @{context}
+    (CASE "t = Leaf" THEN CASE "cl t = R" THEN
+     OBTAIN "max_depth (lsub t) \<le> 2 * black_depth (lsub t) + 1" THEN
+     OBTAIN "max_depth (rsub t) \<le> 2 * black_depth (rsub t) + 1") *} )
+
+setup {* fold add_forward_prfstep [@{thm depth_min}, @{thm depth_max}] *}
+theorem balanced: "is_rbt t \<Longrightarrow> max_depth t \<le> 2 * min_depth t + 1"
+  by (tactic {* auto2s_tac @{context}
+    (OBTAIN "max_depth t \<le> 2 * black_depth t + 1") *})
+setup {* fold del_prfstep_thm [@{thm depth_min}, @{thm depth_max}] *}
+
+subsection {* Definition and basic properties of cl_inv' *}
+
+fun cl_inv' :: "('a, 'b) rbt \<Rightarrow> bool" where
+  "cl_inv' Leaf = True"
+| "cl_inv' (rbt.Node l c k v r) = (cl_inv l \<and> cl_inv r)"
+setup {* fold add_rewrite_rule @{thms cl_inv'.simps} *}
+
+theorem cl_inv_B [forward, backward2]: "rbt.cl t = B \<Longrightarrow> cl_inv' t \<Longrightarrow> cl_inv t" by auto2
+theorem cl_inv_R [forward]:
+  "cl_inv' (rbt.Node l R k v r) \<Longrightarrow> rbt.cl l = B \<Longrightarrow> rbt.cl r = B \<Longrightarrow> cl_inv (rbt.Node l R k v r)" by auto2
+theorem cl_inv_imp [forward]: "cl_inv t \<Longrightarrow> cl_inv' t"
+  by (tactic {* auto2s_tac @{context} (CASE "rbt.cl t = R") *})
+theorem cl_inv'I: "cl_inv l \<Longrightarrow> cl_inv r \<Longrightarrow> cl_inv' (rbt.Node l c k v r)" by auto
+setup {* add_forward_prfstep_cond @{thm cl_inv'I} [with_term "cl_inv' (rbt.Node ?l ?c ?k ?v ?r)"] *}
+
+section {* Tree nodes *}
+
+datatype ('a, 'b) rbt_node =
+  Node (lsub: "('a, 'b) rbt_node ref option") (cl: color) (key: 'a) (val: 'b) (rsub: "('a, 'b) rbt_node ref option")
+
+fun color_encode :: "color \<Rightarrow> nat" where
+  "color_encode B = 0"
+| "color_encode R = 1"
+
+instance color :: heap
+  apply (rule heap_class.intro)
+  apply (rule countable_classI [of "color_encode"])
+  apply (metis color_encode.simps(1) color_encode.simps(2) not_B zero_neq_one)
+  ..
+
+fun rbt_node_encode :: "('a::heap, 'b::heap) rbt_node \<Rightarrow> nat" where
+  "rbt_node_encode (Node l c k v r) = to_nat (l, c, k, v, r)"
+
+instance rbt_node :: (heap, heap) heap
+  apply (rule heap_class.intro)
+  apply (rule countable_classI [of "rbt_node_encode"])
+  apply (case_tac x, simp_all, case_tac y, simp_all)
+  ..
+
+setup {* fold add_rewrite_rule @{thms rbt_node.sel} *}
+theorem rbt_node_constr:
+  "Node l c k v r = Node l' c' k' v' r' \<Longrightarrow> l = l' \<and> c = c' \<and> k = k' \<and> v = v' \<and> r = r'" by simp
+setup {* add_forward_prfstep @{thm rbt_node_constr} *}
+
+fun btree :: "('a::heap, 'b::heap) rbt \<Rightarrow> ('a, 'b) rbt_node ref option \<Rightarrow> assn" where
+  "btree Leaf p = \<up>(p = None)"
+| "btree (rbt.Node lt c k v rt) (Some p) = (\<exists>\<^sub>Alp rp. p \<mapsto>\<^sub>r Node lp c k v rp * btree lt lp * btree rt rp)"
+| "btree (rbt.Node lt c k v rt) None = false"
+setup {* fold add_rewrite_rule @{thms btree.simps} *}
+
+lemma btree_split_iff1 [rewrite]: "btree t None = \<up>(t = Leaf)" by auto2
+
+lemma btree_split_iff2 [forward_ent]:
+  "btree (rbt.Node lt c k v rt) (Some p) \<Longrightarrow>\<^sub>A (\<exists>\<^sub>Alp rp. p \<mapsto>\<^sub>r Node lp c k v rp * btree lt lp * btree rt rp)" by auto2
+
+lemma btree_split_elim:
+  "\<exists>lp rp. h \<Turnstile> p \<mapsto>\<^sub>r Node lp c k v rp * Ql lp rp \<Longrightarrow> h \<Turnstile> p \<mapsto>\<^sub>r Node lp c k v rp * Q \<Longrightarrow>
+   h \<Turnstile> p \<mapsto>\<^sub>r Node lp c k v rp * Ql lp rp" by auto2
+setup {* add_gen_prfstep ("btree_split_elim", forward_descs @{thm btree_split_elim} @ [ShadowFirst]) *}
+
+lemma btree_is_some: "h \<Turnstile> btree (rbt.Node lt c k v rt) q * Qu \<Longrightarrow> q \<noteq> None" by auto2
+setup {* add_forward_prfstep_cond @{thm btree_is_some} [with_cond "?q \<noteq> None"] *}
+
+lemma btree_constr_ent [forward_ent]:
+  "p \<mapsto>\<^sub>r Node lp c k v rp * btree lt lp * btree rt rp \<Longrightarrow>\<^sub>A btree (rbt.Node lt c k v rt) (Some p)" by auto2
+setup {* del_prfstep_thm @{thm btree.simps(2)} *}
+
+lemma btree_prec [sep_prec_thms]:
+  "h \<Turnstile> btree t p * F1 \<Longrightarrow> h \<Turnstile> btree t' p * F2 \<Longrightarrow> t = t'"
+  by (tactic {* auto2s_tac @{context}
+    (INDUCT ("t", Arbitraries ["p", "t'", "F1", "F2"]) THEN CASE "t' = Leaf") *})
+
+theorem btree_some [resolve]: "\<not>h \<Turnstile> btree Leaf (Some p) * Ru" by auto2
+theorem btree_none [match_code_pos_emp]: "btree Leaf None = emp" by auto2
+
+lemma rbt_is_not_leaf:
+  "h \<Turnstile> btree t (Some p) * Qu \<Longrightarrow> t \<noteq> Leaf" by auto2
+setup {* add_forward_prfstep_cond @{thm rbt_is_not_leaf} [with_cond "?t \<noteq> rbt.Node ?lt ?c ?k ?v ?rt"] *}
+
+type_synonym ('a, 'b) btree = "('a, 'b) rbt_node ref option"
+
+section {* Operations *}
+
+subsection {* Basic operations *}
+
+definition tree_empty :: "('a, 'b) btree Heap" where
+  "tree_empty \<equiv> return None"
+declare tree_empty_def [sep_proc_defs]
+
+lemma tree_empty_rule [next_code_pos]:
+  "<emp> tree_empty <btree Leaf>" by auto2
+
+definition tree_is_empty :: "('a, 'b) btree \<Rightarrow> bool Heap" where
+  "tree_is_empty b \<equiv> return (b = None)"
+declare tree_is_empty_def [sep_proc_defs]
+
+lemma tree_is_empty_rule:
+  "<btree t b> tree_is_empty b <\<lambda>r. btree t b * \<up>(r \<longleftrightarrow> t = Leaf)>" by auto2
+
+definition btree_constr :: "('a::heap, 'b::heap) btree \<Rightarrow> color \<Rightarrow> 'a \<Rightarrow> 'b \<Rightarrow> ('a, 'b) btree \<Rightarrow> ('a, 'b) btree Heap" where
+  "btree_constr lp c k v rp = do { p \<leftarrow> ref (Node lp c k v rp); return (Some p) }"
+declare btree_constr_def [sep_proc_defs]
+
+lemma btree_constr_rule [next_code_pos, resolve]:
+  "<btree lt lp * btree rt rp> btree_constr lp c k v rp <btree (rbt.Node lt c k v rt)>" by auto2
+
+partial_function (heap) extract_tree ::
+  "('a::heap, 'b::heap) btree \<Rightarrow> ('a, 'b) rbt Heap" where
+  "extract_tree p = (case p of
+     None \<Rightarrow> return Leaf
+   | Some pp \<Rightarrow> do {
+      t \<leftarrow> !pp;
+      lt \<leftarrow> extract_tree (lsub t);
+      rt \<leftarrow> extract_tree (rsub t);
+      return (rbt.Node lt (cl t) (key t) (val t) rt)
+    })"
+declare extract_tree.simps [sep_proc_defs]
+
+theorem extract_tree_rule [next_code_pos_direct]:
+  "<btree t p> extract_tree p <\<lambda>r. btree t p * \<up>(r = t)>"
+  by (tactic {* auto2s_tac @{context} (INDUCT ("t", Arbitraries ["p"])) *})
+
+definition set_color :: "color \<Rightarrow> ('a::heap, 'b::heap) btree \<Rightarrow> unit Heap" where
+  "set_color c p = (case p of
+    None \<Rightarrow> raise ''set_color''
+  | Some pp \<Rightarrow> do {
+      t \<leftarrow> !pp;
+      pp := Node (lsub t) c (key t) (val t) (rsub t)
+    })"
+declare set_color_def [sep_proc_defs]
+
+theorem set_color_rule [next_code_pos]:
+  "<btree (rbt.Node a c x v b) p>
+   set_color c' p
+   <\<lambda>r. btree (rbt.Node a c' x v b) p>" by auto2
+
+subsection {* Rotation *}
+
+definition btree_rotate_l :: "('a::heap, 'b::heap) btree \<Rightarrow> ('a, 'b) btree Heap" where
+  "btree_rotate_l p = (case p of
+    None \<Rightarrow> raise ''Empty btree''
+  | Some pp \<Rightarrow> do {
+     t \<leftarrow> !pp;
+     (case rsub t of
+        None \<Rightarrow> raise ''Empty rsub''
+      | Some rp \<Rightarrow> do {
+          rt \<leftarrow> !rp;
+          pp := Node (lsub t) (cl t) (key t) (val t) (lsub rt);
+          rp := Node p (cl rt) (key rt) (val rt) (rsub rt);
+          return (rsub t) })})"
+declare btree_rotate_l_def [sep_proc_defs]
+
+lemma btree_rotate_l_rule [next_code_pos]:
+  "<btree (rbt.Node a c1 x v (rbt.Node b c2 y w c)) p>
+   btree_rotate_l p
+   <btree (rbt.Node (rbt.Node a c1 x v b) c2 y w c)>" by auto2
+
+definition btree_rotate_l_at_l :: "('a::heap, 'b::heap) btree \<Rightarrow> unit Heap" where
+  "btree_rotate_l_at_l p = (case p of
+    None \<Rightarrow> raise ''rotate_l_at_l''
+  | Some pp \<Rightarrow> do {
+      t \<leftarrow> !pp;
+      p' \<leftarrow> btree_rotate_l (lsub t);
+      pp := Node p' (cl t) (key t) (val t) (rsub t)
+    })"
+declare btree_rotate_l_at_l_def [sep_proc_defs]
+
+lemma btree_rotate_l_at_l_rule [next_code_pos]:
+  "<btree (rbt.Node (rbt.Node a c2 k2 v2 (rbt.Node b c3 k3 v3 c)) c1 k1 v1 d) p>
+   btree_rotate_l_at_l p
+   <\<lambda>_. btree (rbt.Node (rbt.Node (rbt.Node a c2 k2 v2 b) c3 k3 v3 c) c1 k1 v1 d) p>" by auto2
+
+definition btree_rotate_r :: "('a::heap, 'b::heap) btree \<Rightarrow> ('a, 'b) btree Heap" where
+  "btree_rotate_r p = (case p of
+    None \<Rightarrow> raise ''Empty btree''
+  | Some pp \<Rightarrow> do {
+     t \<leftarrow> !pp;
+     (case lsub t of
+        None \<Rightarrow> raise ''Empty lsub''
+      | Some lp \<Rightarrow> do {
+          lt \<leftarrow> !lp;
+          pp := Node (rsub lt) (cl t) (key t) (val t) (rsub t);
+          lp := Node (lsub lt) (cl lt) (key lt) (val lt) p;
+          return (lsub t) })})"
+declare btree_rotate_r_def [sep_proc_defs]
+
+lemma btree_rotate_r_rule [next_code_pos]:
+  "<btree (rbt.Node (rbt.Node a c1 x v b) c2 y w c) p>
+   btree_rotate_r p
+   <btree (rbt.Node a c1 x v (rbt.Node b c2 y w c))>" by auto2
+
+definition btree_rotate_r_at_r :: "('a::heap, 'b::heap) btree \<Rightarrow> unit Heap" where
+  "btree_rotate_r_at_r p = (case p of
+    None \<Rightarrow> raise ''rotate_r_at_r''
+  | Some pp \<Rightarrow> do {
+      t \<leftarrow> !pp;
+      p' \<leftarrow> btree_rotate_r (rsub t);
+      pp := Node (lsub t) (cl t) (key t) (val t) p'
+    })"
+declare btree_rotate_r_at_r_def [sep_proc_defs]
+
+lemma btree_rotate_r_at_r_rule [next_code_pos]:
+  "<btree (rbt.Node a c1 k1 v1 (rbt.Node (rbt.Node b c2 k2 v2 c) c3 k3 v3 d)) p>
+   btree_rotate_r_at_r p
+   <\<lambda>_. btree (rbt.Node a c1 k1 v1 (rbt.Node b c2 k2 v2 (rbt.Node c c3 k3 v3 d))) p>" by auto2
+
+section {* Balancing *}
+
+definition get_cl :: "('a::heap, 'b::heap) btree \<Rightarrow> color Heap" where
+  "get_cl p = (case p of
+     None \<Rightarrow> return B
+   | Some pp \<Rightarrow> do {
+       t \<leftarrow> !pp;
+       return (cl t)
+     })"
+declare get_cl_def [sep_proc_defs]
+
+theorem get_cl_heap_preserving [sep_heap_presv_thms, heap_presv_thms]:
+  "heap_preserving (get_cl p)"
+  by (tactic {* auto2s_tac @{context} (CASE "p = None") *})
+
+theorem get_cl_rule [next_code_pos_direct]:
+  "<btree t p> get_cl p <\<lambda>r. btree t p * \<up>(r = rbt.cl t)>" by auto2
+
+definition btree_balanceR :: "('a::heap, 'b::heap) btree \<Rightarrow> ('a, 'b) btree Heap" where
+  "btree_balanceR p = (case p of None \<Rightarrow> return None | Some pp \<Rightarrow> do {
+     t \<leftarrow> !pp;
+     if cl t = R then return p
+     else do {
+       cl_r \<leftarrow> get_cl (rsub t);
+       if cl_r = R then do {
+          rt \<leftarrow> !(the (rsub t));
+          cl_lr \<leftarrow> get_cl (lsub rt);
+          cl_rr \<leftarrow> get_cl (rsub rt);
+          if cl_lr = R then do {
+            btree_rotate_r_at_r p;
+            p' \<leftarrow> btree_rotate_l p;
+            t' \<leftarrow> !(the p');
+            set_color B (rsub t');
+            return p'
+          } else if cl_rr = R then do {
+            p' \<leftarrow> btree_rotate_l p;
+            t' \<leftarrow> !(the p');
+            set_color B (rsub t');
+            return p'
+          } else return p }
+       else return p
+     }})"
+declare btree_balanceR_def [sep_proc_defs]
+
+theorem balanceR_bd [next_code_pos]:
+  "<btree t p * \<up>(bd_inv t)>
+   btree_balanceR p
+   <\<lambda>r. \<exists>\<^sub>At'. btree t' r * \<up>(bd_inv t') * \<up>(black_depth t' = black_depth t)>"
+  by auto2
+
+theorem balanceR_cl [next_code_pos]:
+  "<btree (rbt.Node lt B k v rt) p * \<up>(cl_inv lt) * \<up>(cl_inv' rt)>
+   btree_balanceR p
+   <\<lambda>r. \<exists>\<^sub>At'. btree t' r * \<up>(cl_inv t')>"
+  by auto2
+
+definition btree_balance :: "('a::heap, 'b::heap) btree \<Rightarrow> ('a, 'b) btree Heap" where
+  "btree_balance p = (case p of None \<Rightarrow> return None | Some pp \<Rightarrow> do {
+     t \<leftarrow> !pp;
+     if cl t = R then return p
+     else do {
+       cl_l \<leftarrow> get_cl (lsub t);
+       if cl_l = R then do {
+          lt \<leftarrow> !(the (lsub t));
+          cl_rl \<leftarrow> get_cl (rsub lt);
+          cl_ll \<leftarrow> get_cl (lsub lt);
+          if cl_rl = R then do {
+            btree_rotate_l_at_l p;
+            p' \<leftarrow> btree_rotate_r p;
+            t' \<leftarrow> !(the p');
+            set_color B (lsub t');
+            return p'
+          } else if cl_ll = R then do {
+            p' \<leftarrow> btree_rotate_r p;
+            t' \<leftarrow> !(the p');
+            set_color B (lsub t');
+            return p'
+          } else btree_balanceR p }
+       else do {
+         p' \<leftarrow> btree_balanceR p;
+         return p'
+       }
+     }})"
+declare btree_balance_def [sep_proc_defs]
+
+theorem balance_bd [next_code_pos]:
+  "<btree t p * \<up>(bd_inv t)>
+   btree_balance p
+   <\<lambda>r. \<exists>\<^sub>At'. btree t' r * \<up>(bd_inv t') * \<up>(black_depth t' = black_depth t)>"
+   by auto2
+
+theorem balance_cl1 [next_code_pos]:
+  "<btree (rbt.Node lt B k v rt) p * \<up>(cl_inv' lt) * \<up>(cl_inv rt)>
+   btree_balance p
+   <\<lambda>r. \<exists>\<^sub>At'. btree t' r * \<up>(cl_inv t')>"
+   by auto2
+
+theorem balance_cl2 [next_code_pos]:
+  "<btree (rbt.Node lt B k v rt) p * \<up>(cl_inv lt) * \<up>(cl_inv' rt)>
+   btree_balance p
+   <\<lambda>r. \<exists>\<^sub>At'. btree t' r * \<up>(cl_inv t')>"
+   by auto2
+
+theorem balanceR_non_leaf [next_code_pos]:
+  "<btree (rbt.Node lt c k v rt) p>
+    btree_balanceR p
+   <\<lambda>r. \<exists>\<^sub>At'. btree t' r * \<up>(t' \<noteq> Leaf)>"
+   by auto2
+
+theorem balance_non_leaf [next_code_pos]:
+  "<btree (rbt.Node lt c k v rt) p>
+    btree_balance p
+   <\<lambda>r. \<exists>\<^sub>At'. btree t' r * \<up>(t' \<noteq> Leaf)>"
+   by auto2
+
+theorem balance_on_R [next_code_pos]:
+  "<btree (rbt.Node lt R k v rt) p>
+   btree_balance p
+   <\<lambda>r. \<exists>\<^sub>At'. btree t' r * \<up>(t' = rbt.Node lt R k v rt)>" by auto2
+
+section {* ins function *}
+
+partial_function (heap) rbt_ins ::
+  "'a::{heap,ord} \<Rightarrow> 'b::heap \<Rightarrow> ('a, 'b) btree \<Rightarrow> ('a, 'b) btree Heap" where
+  "rbt_ins k v p = (case p of
+     None \<Rightarrow> btree_constr None R k v None
+   | Some pp \<Rightarrow> do {
+      t \<leftarrow> !pp;
+      (if k = key t then do {
+         pp := Node (lsub t) (cl t) k v (rsub t);
+         return (Some pp) }
+       else if k < key t then do {
+         q \<leftarrow> rbt_ins k v (lsub t);
+         pp := Node q (cl t) (key t) (val t) (rsub t);
+         btree_balance p }
+       else do {
+         q \<leftarrow> rbt_ins k v (rsub t);
+         pp := Node (lsub t) (cl t) (key t) (val t) q;
+         btree_balance p })} )"
+declare rbt_ins.simps [sep_proc_defs]
+
+theorem ins_non_leaf [next_code_pos]:
+  "<btree t p> rbt_ins k v p <\<lambda>r. \<exists>\<^sub>At'. btree t' r * \<up>(t' \<noteq> Leaf)>"
+   by (tactic {* auto2s_tac @{context} (INDUCT ("t", Arbitraries ["p"])) *})
+
+theorem ins_bd [next_code_pos]:
+  "<btree t p * \<up>(bd_inv t)>
+   rbt_ins k v p
+   <\<lambda>r. \<exists>\<^sub>At'. btree t' r * \<up>(bd_inv t') * \<up>(black_depth t' = black_depth t)>"
+   by (tactic {* auto2s_tac @{context} (
+     INDUCT ("t", Arbitraries ["p"]) THEN CASE "rbt.cl t = R") *})
+
+theorem ins_cl [next_code_pos]:
+  "<btree t p * \<up>(cl_inv t)>
+   rbt_ins k v p
+   <\<lambda>r. \<exists>\<^sub>At'. btree t' r * \<up>(if rbt.cl t = B then cl_inv t' else rbt.cl t' = R \<and> cl_inv' t')>"
+   by (tactic {* auto2s_tac @{context} (INDUCT ("t", Arbitraries ["p"])) *})
+
+section {* Insert function *}
+
+definition rbt_insert :: "'a::{heap,ord} \<Rightarrow> 'b::heap \<Rightarrow> ('a, 'b) btree \<Rightarrow> ('a, 'b) btree Heap" where
+  "rbt_insert k v p = do {
+    p' \<leftarrow> rbt_ins k v p;
+    set_color B p';
+    return p' }"
+declare rbt_insert_def [sep_proc_defs]
+
+theorem insert_is_rbt [next_code_pos]:
+  "<btree t p * \<up>(is_rbt t)>
+   rbt_insert k v p
+   <\<lambda>r. \<exists>\<^sub>At'. btree t' r * \<up>(is_rbt t')>" by auto2
+
+(* insert_is_rbt is all we need, so we can clear out bd and cl properties. *)
+setup {* fold del_prfstep_thm [
+  @{thm balanceR_bd}, @{thm balanceR_cl}, @{thm balance_bd},
+  @{thm balance_cl1}, @{thm balance_cl2}, @{thm ins_bd}, @{thm ins_cl}] *}
+
+section {* Set of keys and mapping associated to an RBT, sortedness on RBT *}
+
+fun rbt_key_set :: "('a, 'b) rbt \<Rightarrow> 'a set" where
+  "rbt_key_set Leaf = {}"
+| "rbt_key_set (rbt.Node lt c k v rt) = {k} \<union> rbt_key_set lt \<union> rbt_key_set rt"
+setup {* fold add_rewrite_rule @{thms rbt_key_set.simps} *}
+
+fun rbt_sorted :: "('a::linorder, 'b) rbt \<Rightarrow> bool" where
+  "rbt_sorted Leaf = True"
+| "rbt_sorted (rbt.Node lt c k v rt) =
+   ((\<forall>x\<in>rbt_key_set lt. x < k) \<and> (\<forall>x\<in>rbt_key_set rt. k < x) \<and> rbt_sorted lt \<and> rbt_sorted rt)"
+setup {* fold add_rewrite_rule @{thms rbt_sorted.simps} *}
+
+lemma rbt_sorted_on_left [forward]:
+  "rbt_sorted (rbt.Node (rbt.Node a c1 x v b) c2 y w c) \<Longrightarrow> x < y" by auto2 
+
+lemma rbt_sorted_on_right [forward]:
+  "rbt_sorted (rbt.Node a c1 x v (rbt.Node b c2 y w c)) \<Longrightarrow> x < y" by auto2
+
+fun tree_map :: "('a::linorder, 'b) rbt \<Rightarrow> ('a, 'b) map" where
+  "tree_map Leaf = Map (\<lambda>x. None)"
+| "tree_map (rbt.Node lt c k v rt) = binary_map k v (tree_map lt) (tree_map rt)"
+setup {* fold add_rewrite_rule @{thms tree_map.simps} *}
+
+(* Sortedness and preservation of set of keys is best proved by
+   introducing in-order traversal. *)
+fun rbt_in_traverse :: "('a, 'b) rbt \<Rightarrow> 'a list" where
+  "rbt_in_traverse Leaf = []"
+| "rbt_in_traverse (rbt.Node lt c k v rt) = (rbt_in_traverse lt) @ [k] @ (rbt_in_traverse rt)"
+setup {* fold add_rewrite_rule @{thms rbt_in_traverse.simps} *}
+
+theorem rbt_in_traverse_non_empty:
+  "rbt_in_traverse (rbt.Node lt c k v rt) \<noteq> []" by auto2
+
+theorem inorder_preserve_set [rewrite_bidir]:
+  "set (rbt_in_traverse t) = rbt_key_set t" by auto2
+
+fun strict_sorted :: "'a::linorder list \<Rightarrow> bool" where
+  "strict_sorted [] = True"
+| "strict_sorted (x # ys) = ((\<forall>y\<in>set ys. x < y) \<and> strict_sorted ys)"
+setup {* fold add_rewrite_rule @{thms strict_sorted.simps} *}
+
+theorem strict_sorted_single [resolve]: "strict_sorted [x]" by auto2
+setup {* del_prfstep_thm @{thm strict_sorted.simps(2)} #>
+  add_rewrite_rule_cond @{thm strict_sorted.simps(2)} [with_cond "?ys \<noteq> []"] *}
+
+theorem strict_sorted_append [rewrite]:
+  "strict_sorted (xs @ ys) =
+    ((\<forall>x y. x \<in> set xs \<longrightarrow> y \<in> set ys \<longrightarrow> x < y) \<and> strict_sorted xs \<and> strict_sorted ys)"
+  by (tactic {* auto2s_tac @{context} (INDUCT ("xs", [])) *})
+
+theorem inorder_sorted [rewrite_bidir]:
+  "strict_sorted (rbt_in_traverse t) = rbt_sorted t" by auto2
+setup {* del_prfstep_thm @{thm strict_sorted_append} *}
+
+theorem balanceR_in_traverse [next_code_pos]:
+  "<btree t p>
+   btree_balanceR p
+   <\<lambda>r. \<exists>\<^sub>At'. btree t' r * \<up>(rbt_in_traverse t' = rbt_in_traverse t)>"
+  by auto2
+
+theorem balance_in_traverse [next_code_pos]:
+  "<btree t p>
+   btree_balance p
+   <\<lambda>r. \<exists>\<^sub>At'. btree t' r * \<up>(rbt_in_traverse t' = rbt_in_traverse t)>"
+  by auto2
+
+declare btree_balance_def [sep_proc_defs del]
+theorem balance_sorted [next_code_pos]:
+  "<btree t p * \<up>(rbt_sorted t)>
+   btree_balance p
+   <\<lambda>r. \<exists>\<^sub>At'. btree t' r * \<up>(rbt_sorted t')>"
+  by auto2
+
+theorem balance_key_set [next_code_pos]:
+  "<btree t p>
+   btree_balance p
+   <\<lambda>r. \<exists>\<^sub>At'. btree t' r * \<up>(rbt_key_set t' = rbt_key_set t)>"
+  by auto2
+declare btree_balance_def [sep_proc_defs]
+
+theorem ins_key_set [next_code_pos]:
+  "<btree t p>
+   rbt_ins k v p
+   <\<lambda>r. \<exists>\<^sub>At'. btree t' r * \<up>(rbt_key_set t' = {k} \<union> rbt_key_set t)>"
+  by (tactic {* auto2s_tac @{context} (INDUCT ("t", Arbitraries ["p"])) *})
+
+theorem ins_sorted [next_code_pos]:
+  "<btree t p * \<up>(rbt_sorted t)>
+   rbt_ins k v p
+   <\<lambda>r. \<exists>\<^sub>At'. btree t' r * \<up>(rbt_sorted t')>"
+  by (tactic {* auto2s_tac @{context} (INDUCT ("t", Arbitraries ["p"])) *})
+
+theorem insert_key_set [next_code_pos]:
+  "<btree t p>
+   rbt_insert k v p
+   <\<lambda>r. \<exists>\<^sub>At'. btree t' r * \<up>(rbt_key_set t' = {k} \<union> rbt_key_set t)>"
+  by auto2
+
+theorem insert_sorted [next_code_pos]:
+  "<btree t p * \<up>(rbt_sorted t)>
+   rbt_insert k v p
+   <\<lambda>r. \<exists>\<^sub>At'. btree t' r * \<up>(rbt_sorted t')>"
+  by auto2
+
+(* Finally, we prove effect of operations on mapping *)
+
+lemma btree_rotate_preserves_map:
+  "x < y \<Longrightarrow> tree_map (rbt.Node a c1 x v (rbt.Node b c2 y w c)) =
+   tree_map (rbt.Node (rbt.Node a c3 x v b) c4 y w c)" by auto2
+setup {* add_forward_prfstep_cond @{thm btree_rotate_preserves_map}
+  [with_term "rbt.Node ?a ?c1.0 ?x ?v (rbt.Node ?b ?c2.0 ?y ?w ?c)",
+   with_term "rbt.Node (rbt.Node ?a ?c3.0 ?x ?v ?b) ?c4.0 ?y ?w ?c"] *}
+
+theorem balanceR_map [next_code_pos]:
+  "<btree t p * \<up>(rbt_sorted t)>
+   btree_balanceR p
+   <\<lambda>r. \<exists>\<^sub>At'. btree t' r * \<up>(tree_map t' = tree_map t)>"
+  by auto2
+
+theorem balance_map [next_code_pos, code_pos_create_case]:
+  "<btree t p * \<up>(rbt_sorted t)>
+   btree_balance p
+   <\<lambda>r. \<exists>\<^sub>At'. btree t' r * \<up>(tree_map t' = tree_map t)>"
+  by auto2
+
+theorem ins_map [next_code_pos]:
+  "<btree t p * \<up>(rbt_sorted t)>
+   rbt_ins k v p
+   <\<lambda>r. \<exists>\<^sub>At'. btree t' r * \<up>(tree_map t' = (tree_map t) {k \<rightarrow> v})>"
+  by (tactic {* auto2s_tac @{context} (INDUCT ("t", Arbitraries ["p"])) *})
+
+theorem insert_map [next_code_pos]:
+  "<btree t p * \<up>(rbt_sorted t)>
+   rbt_insert k v p
+   <\<lambda>r. \<exists>\<^sub>At'. btree t' r * \<up>(tree_map t' = (tree_map t) {k \<rightarrow> v})>"
+  by auto2
+
+section {* Outer interface *}
+
+definition rbt_set :: "'a set \<Rightarrow> ('a::{heap,linorder}, 'b::heap) rbt_node ref option \<Rightarrow> assn" where
+  "rbt_set S p = (\<exists>\<^sub>At. btree t p * \<up>(is_rbt t) * \<up>(rbt_sorted t) * \<up>(S = rbt_key_set t))"
+setup {* add_rewrite_rule @{thm rbt_set_def} *}
+
+definition rbt_map :: "('a, 'b) map \<Rightarrow> ('a::{heap,linorder}, 'b::heap) rbt_node ref option \<Rightarrow> assn" where
+  "rbt_map M p = (\<exists>\<^sub>At. btree t p * \<up>(is_rbt t) * \<up>(rbt_sorted t) * \<up>(M = tree_map t))"
+setup {* add_rewrite_rule @{thm rbt_map_def} *}
+
+declare tree_empty_def [sep_proc_defs del]
+
+lemma rbt_empty_rule1:
+  "<emp> tree_empty <rbt_set {}>" by auto2
+
+lemma rbt_empty_rule2:
+  "<emp> tree_empty <rbt_map empty_map>" by auto2
+
+declare rbt_insert_def [sep_proc_defs del]
+
+lemma rbt_insert_rule1:
+  "<rbt_set S b> rbt_insert k v b <rbt_set ({k} \<union> S)>" by auto2
+
+lemma rbt_insert_rule2:
+  "<rbt_map M b> rbt_insert k v b <rbt_map (M {k \<rightarrow> v})>" by auto2
+
+end
